\documentclass[11pt]{article}
\usepackage{amsmath}
\begin{document}

\section{DIT-Split Radix}

\[X[k] = \underbrace{\sum_{n=0}^{N/2-1} x[2n] W_{N/2}^{nk}}_{\text{DFT}\{x[2n]\}}
       + W_N^k \underbrace{\sum_{n=0}^{N/4-1} x[4n+1] W_{N/4}^{nk}}_{\text{DFT}\{x[4n+1]\}}
       + W_N^{3k} \underbrace{\sum_{n=0}^{N/4-1} x[4n+3] W_{N/4}^{nk}}_{\text{DFT}\{x[4n+3]\}}\]

\paragraph{Sub DFTs Remain Unchanged}

\[\begin{split}
W_{N/4}^{n(k+N/4)} & = e^{-j\frac{2\pi}{N/4}n(k+N/4)} \\
& = e^{-j\frac{2\pi}{N/4}nk} \underbrace{e^{-j\frac{2\pi}{N/4}n(N/4)}}_{ e^{-j2\pi n} = 1} \\
& = W_{N/4}^{nk}
\end{split}\]

\[W_{N/4}^{n(k+N/2)} = W_{N/4}^{nk}\]
\[W_{N/4}^{n(k+3N/4)} = W_{N/4}^{nk}\]
\[W_{N/2}^{n(k+N/2)} = W_{N/2}^{nk}\]

\paragraph{Twiddle Factors}

\[\begin{split}
W_N^{k+N/4} & = e^{-j\frac{2\pi}{N}(k+N/4)} \\
& = e^{-j\frac{2\pi}{N}k} \underbrace{e^{-j\frac{2\pi}{N}(N/4)}}_{ e^{-j\frac{\pi}{2}} = -j} \\
& = -j W_{N}^k
\end{split}\]

\[W_N^{k+N/2} = -W_N^k\]
\[W_N^{k+3N/4} = W_N^{k+N/2} W_N^{N/4} = W_N^{k+N/4} = j W_{N}^k\]

\bigskip

\[W_N^{3(k+N/4)} = W_N^{3k} W_N^{3N/4} = j W_N^{3k}\]
\[W_N^{3(k+N/2)} = W_N^{3k} W_N^{3N/2} = -W_N^{3k}\]
\[W_N^{3(k+3N/4)} = W_N^{3k} W_N^{3N/4} W_N^{3N/2} = -j W_N^{3k}\]

\paragraph{The Complete Formula}

\[\begin{split}
  X[k] & = X_1[k] + W_N^k X_2[k] + W_N^{3k} X_3[k]\\
  X[k + N/4] & = X_1[k + N/4] - jW_N^k X_2[k] + jW_N^{3k} X_3[k] \\
  X[k + N/2] & = X_1[k] - W_N^k X_2[k] - W_N^{3k} X_3[k] \\
  X[k + 3N/4] & = X_1[k + N/4] + jW_N^k X_2[k] - jW_N^{3k} X_3[k] \\
\end{split}\]

\paragraph{Rearranged Formula}

\[\begin{split}
  X[k] & = X_1[k] + \left(W_N^k X_2[k] + W_N^{3k} X_3[k]\right)\\
  X[k + N/4] & = X_1[k + N/4] - \left(jW_N^k X_2[k] - jW_N^{3k} X_3[k]\right) \\
  X[k + N/2] & = X_1[k] - \left(W_N^k X_2[k] + W_N^{3k} X_3[k]\right) \\
  X[k + 3N/4] & = X_1[k + N/4] + \left(jW_N^k X_2[k] - jW_N^{3k} X_3[k]\right) \\
\end{split}\]

\section{8-Point Split Radix}

\[\begin{split}
  X[0] & = X_1[0] + X_2[0] + X_3[0]\\
  X[1] & = X_1[1] + W_8 X_2[1] + W_8^3 X_3[1]\\
  X[2] & = X_1[2] - j X_2[0] + j X_3[0]\\
  X[3] & = X_1[3] - jW_8 X_2[1] + W_8^3 X_3[1]\\
  X[4] & = X_1[0] - X_2[0] - X_3[0]\\
  X[5] & = X_1[1] - W_8 X_2[1] - W_8^3 X_3[1]\\
  X[6] & = X_1[2] + j X_2[0] - j X_3[0]\\
  X[7] & = X_1[3] + jW_8 X_2[1] - j W_8^3 X_3[1]\\
\end{split}\]
\end{document}
